Blanc/Bits.lean
@@ -1,0 +1,1550 @@
+import Mathlib.Data.Nat.Basic
+import Mathlib.Data.List.Lemmas
+import Mathlib.Util.Notation3
+import Mathlib.Data.Vector.Basic
+import Elevm.Basic
+
+instance : @Zero Bool := ⟨false⟩
+instance : @One Bool := ⟨true⟩
+
+def Bool.toChar : Bool → Char
+  | 0 => '0'
+  | 1 => '1'
+
+theorem Bool.zero_or_one (x : Bool) : x = 0 ∨ x = 1 := by
+  cases x
+  · left; rfl
+  · right; rfl
+
+theorem not_true_lt {b} : ¬ true < b := by simp [LT.lt]
+theorem Bool.zero : 0 = false := rfl
+theorem Bool.one : 1 = true := rfl
+
+inductive Bits : ℕ → Type
+  | nil : Bits 0
+  | cons : ∀ {n : ℕ}, Bool → Bits n → Bits (n + 1)
+
+abbrev Addr := Bits 160
+abbrev Word := Bits 256
+
+notation "⦃⦄" => Bits.nil
+
+infixr:70 " +> " => Bits.cons
+
+syntax "⦃" withoutPosition(term,*,?) "⦄"  : term
+macro_rules
+  | `(⦃$l,*⦄) => `(expand_foldr% (h t => Bits.cons h t) Bits.nil [$(.ofElems l),*])
+
+abbrev Byte := Bits 8
+abbrev Bytes : Type := List Byte
+
+def Bits.toChars : ∀ {n}, Bits n → List Char
+  | 0, ⦃⦄ => []
+  | _ + 1, x +> xs => Bool.toChar x :: xs.toChars
+
+def Bits.toString {n} (bs : Bits n) : String := ⟨Bits.toChars bs⟩
+
+instance {n} : Repr (Bits n) := ⟨λ bs _ => Bits.toString bs⟩
+
+def Bits.not : ∀ {n}, Bits n → Bits n
+  | 0, ⦃⦄ => ⦃⦄
+  | _, (x +> xs) => x.not +> xs.not
+
+notation "~" => Bits.not
+
+instance {n} : Complement (Bits n) := ⟨Bits.not⟩
+
+def Bits.zipWith (f : Bool → Bool → Bool) : ∀ {n}, Bits n → Bits n → Bits n
+  | 0, ⦃⦄, ⦃⦄ => ⦃⦄
+  | _, x +> xs, y +> ys => f x y +> (zipWith f xs ys)
+
+def Bits.and {n} : Bits n → Bits n → Bits n := zipWith Bool.and
+
+instance {n} : HAnd (Bits n) (Bits n) (Bits n) := ⟨Bits.and⟩
+
+def Bits.or {n} : Bits n → Bits n → Bits n := zipWith Bool.or
+def Bits.xor {n} : Bits n → Bits n → Bits n := zipWith Bool.xor
+
+theorem Bits.cons_and_cons {n} {xs ys : Bits n} {x y} :
+  and (x +> xs) (y +> ys) = .and x y +> and xs ys := rfl
+
+def Bits.lt : ∀ {n : ℕ}, Bits n → Bits n → Prop
+  | 0, ⦃⦄, ⦃⦄ => False
+  | _, x +> xs, y +> ys => x < y ∨ (x = y ∧ lt xs ys)
+
+def Bits.lt' : ∀ {n : ℕ}, Bits n → Bits n → Bool
+  | 0, ⦃⦄, ⦃⦄ => false
+  | _, x +> xs, y +> ys => (!x && y) || (x == y && lt' xs ys)
+
+instance {n} : @LT (Bits n) := ⟨Bits.lt⟩
+
+theorem Bits.cons_lt_cons {n} {x y} {xs ys : Bits n} :
+    x +> xs < y +> ys ↔ (x < y ∨ (x = y ∧ xs < ys)) := Iff.refl _
+
+theorem Bits.cons_eq_cons {n} {x y} {xs ys : Bits n} :
+    x +> xs = y +> ys ↔ (x = y ∧ xs = ys) := by simp
+
+instance {n} {xs ys : Bits n} : Decidable (xs < ys) := by
+  induction n with
+  | zero =>
+    cases xs; cases ys; simp [LT.lt, Bits.lt]
+    apply Decidable.isFalse not_false
+  | succ n ih =>
+    match xs, ys with
+    | x +> xs, y +> ys =>
+      cases x <;> cases y <;>
+      simp [Bits.cons_lt_cons, not_true_lt] <;>
+      try {apply ih}; apply instDecidableTrue; apply instDecidableFalse
+
+def Bits.le : ∀ {n : ℕ}, Bits n → Bits n → Prop
+  | 0, ⦃⦄, ⦃⦄ => True
+  | _, x +> xs, y +> ys => x < y ∨ (x = y ∧ le xs ys)
+
+instance {n} : @LE (Bits n) := ⟨Bits.le⟩
+
+theorem Bits.cons_le_cons {n} {xs ys : Bits n} {x y} :
+    x +> xs ≤ y +> ys ↔ (x < y ∨ (x = y ∧ xs ≤ ys)) := Iff.refl _
+
+instance {n : ℕ} (xs ys : Bits n) : Decidable (xs = ys) := by
+  induction n with
+  | zero => cases xs; cases ys; apply Decidable.isTrue rfl
+  | succ n ih =>
+    match xs, ys with
+    | x +> xs, y +> ys =>
+      rw [Bits.cons_eq_cons]; apply instDecidableAnd
+
+
+instance {n : ℕ} (xs ys : Bits n) : Decidable (xs ≤ ys) := by
+  induction n with
+  | zero =>
+    cases xs; cases ys;
+    apply Decidable.isTrue; constructor
+  | succ n =>
+    match xs, ys with
+    | x +> xs, y +> ys =>
+      rw [Bits.cons_le_cons]; apply instDecidableOr
+
+def Bits.Slt : ∀ {n : ℕ}, Bits n → Bits n → Prop
+  | 0, ⦃⦄, ⦃⦄ => False
+  | _ + 1, x +> xs, y +> ys => y < x ∨ (x = y ∧ xs < ys)
+
+infix:70 " ±< " => Bits.Slt
+
+theorem Bits.singleton_slt_singleton {x y : Bool} :
+    ⦃x⦄ ±< ⦃y⦄ ↔ (x = 1 ∧ y = 0) := by
+  cases x <;> cases y <;>
+  simp [Bool.zero, Bool.one, Bits.Slt, LT.lt] <;>
+  try {intro hc; cases hc}
+
+def Bits.Sgt {n : ℕ} (xs ys : Bits n) : Prop := Slt ys xs
+
+infix:70 " ±> " => Bits.Sgt
+
+def Bits.toNat : ∀ {n : ℕ}, Bits n → Nat
+  | 0, ⦃⦄ => 0
+  | n + 1, x +> xs => (cond x (2 ^ n) 0) + xs.toNat
+
+def Bits.zero : ∀ n : ℕ, Bits n
+  | 0 => ⦃⦄
+  | n + 1 => 0 +> zero n
+
+instance {n} : Inhabited (Bits n) := ⟨Bits.zero n⟩
+instance {n} : @Zero (Bits n) := ⟨Bits.zero n⟩
+instance : @Zero Byte := ⟨Bits.zero 8⟩
+
+def Bits.max : ∀ n : ℕ, Bits n
+  | 0 => ⦃⦄
+  | n + 1 => 1 +> max n
+
+def Bits.one : ∀ n : ℕ, Bits n
+  | 0 => ⦃⦄
+  | 1 => ⦃1⦄
+  | n + 2 => 0 +> one (n + 1)
+
+instance {n} : @One (Bits n) := ⟨Bits.one n⟩
+
+def Bits.rec2 {μ : ∀ n, Bits n → Bits n → Sort u}
+    (nil : μ 0 ⦃⦄ ⦃⦄)
+    (cons : ∀ {n} x xs y ys, μ n xs ys → μ (n + 1) (x +> xs) (y +> ys))
+    {n} (xs ys : Bits n) : μ n xs ys := by
+  induction n with
+  | zero => cases xs; cases ys; exact nil
+  | succ n ih =>
+    match xs, ys with
+    | x +> xs, y +> ys => apply cons; apply ih
+
+def Bits.isMax : ∀ {n}, Bits n → Bool
+  | 0, ⦃⦄ => true
+  | _ + 1, x +> xs => x && xs.isMax
+
+def Bits.succ : ∀ {n}, Bits n →  Bits n
+  | 0, ⦃⦄ => ⦃⦄
+  | _ + 1, x +> xs => (x != xs.isMax) +> xs.succ
+
+def Bits.incr {n} : Bool → Bits n → Bits n
+  | false => id
+  | true => Bits.succ
+
+def Overflow {n : ℕ} (xs ys : Bits n) : Prop := 2 ^ n ≤ xs.toNat + ys.toNat
+
+def overflow : ∀ {n : ℕ}, Bits n → Bits n → Bool
+  | 0, ⦃⦄, ⦃⦄ => false
+  | _ + 1, x +> xs, y +> ys => (x && y) || ((x != y) && overflow xs ys)
+
+theorem overflow_comm :
+    ∀ {n : ℕ} (xs ys : Bits n), overflow xs ys = overflow ys xs := by
+  apply Bits.rec2
+  · rfl
+  · intro n x xs y ys ih; simp only [overflow, bne]
+    rw [Bool.and_comm, Bool.beq_comm, ih];
+
+def Bits.add : ∀ {n : ℕ}, Bits n → Bits n → Bits n
+  | 0, ⦃⦄, ⦃⦄ => ⦃⦄
+  | _ + 1, x +> xs, y +> ys =>
+    ((x != y) != overflow xs ys) +> (add xs ys)
+
+infix:55 " ↟ " => Overflow
+
+def Nof {n : ℕ} (xs ys : Bits n) : Prop := xs.toNat + ys.toNat < 2 ^ n
+
+def Bits.nof_iff_not_overflow {n : ℕ} (xs ys : Bits n) : Nof xs ys ↔ ¬ xs ↟ ys := by
+  simp [Overflow, Nof]
+
+def Bits.sub {n} : Bits n → Bits n → Bits n
+  | ⦃⦄, ⦃⦄ => ⦃⦄
+  | x +> xs, y +> ys => ((x != y) != lt' xs ys) +> sub xs ys
+
+instance {n} : HAdd (Bits n) (Bits n) (Bits n) := ⟨Bits.add⟩
+instance {n} : Add (Bits n) := ⟨Bits.add⟩
+
+instance {n} : HSub (Bits n) (Bits n) (Bits n) := ⟨Bits.sub⟩
+instance {n} : Sub (Bits n) := ⟨Bits.sub⟩
+
+theorem Bits.faux :
+  ∀ {n} {xs ys : Bits n}, lt' xs ys = overflow (xs - ys) ys := by
+  apply rec2
+  · simp [lt']; rfl
+  · intro n x xs y ys ih
+    simp only [lt', HSub.hSub, Bits.sub, overflow]
+    conv => rhs; rhs; rhs; apply ih.symm
+    cases (lt' xs ys) <;> cases y <;> simp
+
+theorem Bits.lt_irrefl {n} {xs : Bits n} : ¬ xs < xs := by
+  intro h;
+  induction n with
+  | zero => cases xs; cases h
+  | succ n ih =>
+    match xs with
+    | x +> xs =>
+      rcases h with h | h
+      · apply Bool.lt_irrefl _ h
+      · apply ih h.right
+
+theorem Bits.nil_eq_nil {x y : Bits 0} : x = y := by cases x; cases y; rfl
+theorem Bits.eq_nil {x : Bits 0} : x = ⦃⦄ := nil_eq_nil
+
+theorem Bits.cons_sub_cons {n} {x y} {xs ys : Bits n} :
+  (x +> xs) - (y +> ys) = ((x != y) != lt' xs ys) +> (xs - ys) := rfl
+
+theorem Bits.cons_add_cons {n} {x y} {xs ys : Bits n} :
+    (x +> xs) + (y +> ys) = ((x != y) != overflow xs ys) +> (xs + ys) := rfl
+
+def Bits.snoc : ∀ {n}, Bits n → Bool → Bits (n + 1)
+  | 0, ⦃⦄, y => ⦃y⦄
+  | _ + 1, x +> xs, y => x +> (xs.snoc y)
+
+def Bits.shlo : ∀ {n}, Bits n → Bool → Bits n
+  | 0, ⦃⦄, _ => ⦃⦄
+  | _ + 1, _ +> xs, y => Bits.snoc xs y
+
+def Bits.shl : Nat → ∀ {n}, Bits n → Bits n
+  | 0, _, xs => xs
+  | m + 1, _, xs => shlo (xs.shl m) 0
+
+def Bits.prefixLe : ∀ {m n}, m ≤ n → Bits n → Bits m
+| 0, _, _, _ => ⦃⦄
+| m + 1, 0, h, _ => (Nat.not_succ_le_zero m h).elim
+| _ + 1, _ + 1, h, x +> xs =>
+  x +> prefixLe (Nat.le_of_succ_le_succ h) xs
+
+def Bits.shiftRightCore (sign : Bool) :
+  Nat → ∀ {m n}, m ≤ n → Bits n → Bits m
+  | _, 0, _, _, _ => ⦃⦄
+  | 0, _, _, h, xs => prefixLe h xs
+  | k + 1, m + 1, n, h, xs =>
+    sign +> @shiftRightCore sign k m n (le_trans (Nat.le_succ _) h) xs
+
+def Bits.shr (m : Nat) {n} (xs : Bits n) : Bits n :=
+  shiftRightCore 0 m (le_refl n) xs
+
+def Bits.sar (m : Nat) : ∀ {n}, Bits n → Bits n
+  | 0, ⦃⦄ => ⦃⦄
+  | _ + 1, x +> xs =>
+    shiftRightCore x m (le_refl _) (x +> xs)
+
+def Bits.isNeg : ∀ {n : ℕ}, Bits n → Bool
+  | 0, _ => false
+  | _ + 1, x +> _ => x
+
+def Bits.neg {n : ℕ} (xs : Bits n) : Bits n := (~ xs).succ
+
+def Bits.append : ∀ {m n}, Bits m → Bits n → Bits (n + m)
+  | 0, _, ⦃⦄, ys => ys
+  | _ + 1, _, x +> xs, ys => x +> append xs ys
+
+instance {m n} : HAppend (Bits m) (Bits n) (Bits (n + m)) := ⟨Bits.append⟩
+
+theorem Bits.cons_append {m n} {x} {xs : Bits m} {ys : Bits n} :
+    (x +> xs) ++ ys = x +> (xs ++ ys) := by rfl
+
+theorem Bits.append_and_append {m n} {xs₀ ys₀ : Bits m} {xs₁ ys₁ : Bits n} :
+    and (xs₀ ++ xs₁) (ys₀ ++ ys₁) = and xs₀ ys₀ ++ and xs₁ ys₁ := by
+  induction m with
+  | zero => cases xs₀; cases ys₀; rfl
+  | succ n ih =>
+    match xs₀, ys₀ with
+    | _ +> _, _ +> _ => simp [cons_append, cons_and_cons, ih]
+
+def Bits.mulCore {m} : ∀ {n}, Bits m → Bits n → Bits m
+  | 0, _, ⦃⦄ => 0
+  | _ + 1, xs, 0 +> ys => mulCore xs ys
+  | n + 1, xs, 1 +> ys => shl n xs + mulCore xs ys
+
+def Bits.mul {n} (xs ys : Bits n) : Bits n := mulCore xs ys
+
+instance {n} : HMul (Bits n) (Bits n) (Bits n) := ⟨Bits.mul⟩
+
+-- divMod acc pfx xs ys
+-- assumes: pfx < ys
+def divMod : ∀ {m n : ℕ}, Bits n → Bits m → Bits n → (Bits m × Bits n)
+  | 0, _, pfx, ⦃⦄, _ => (0, pfx)
+  | _ + 1, _, pfx, x +> xs, ys =>
+    let pfx' := Bits.shlo pfx x
+    if ys ≤ pfx'
+    then let (div, mod) := divMod (pfx' - ys) xs ys
+         (1 +> div, mod)
+    else let (div, mod) := divMod pfx' xs ys
+         (0 +> div, mod)
+
+def Bits.div {n} (xs ys : Bits n) : Bits n :=
+  if ys = 0 then 0 else (divMod 0 xs ys).fst
+
+def Bits.mod {n} (xs ys : Bits n) : Bits n :=
+  if ys = 0 then 0 else (divMod 0 xs ys).snd
+
+instance {n} : HDiv (Bits n) (Bits n) (Bits n) := ⟨Bits.div⟩
+instance {n} : HMod (Bits n) (Bits n) (Bits n) := ⟨Bits.mod⟩
+instance {n} : Mod (Bits n) := ⟨Bits.mod⟩
+
+-- minimum possible value in 2's complement
+def Bits.smin : ∀ {n : ℕ}, Bits n
+  | 0 => ⦃⦄
+  | _ + 1 => 1 +> 0
+
+
+def Bits.negOne {n : ℕ} : Bits n := max _
+
+def Bits.sdiv {n : ℕ} (xs ys : Bits n) : Bits n :=
+  if ys = 0
+  then 0
+  else if xs = smin ∧ ys = negOne
+       then smin
+       else match (isNeg xs, isNeg ys) with
+            | (0, 0) => xs / ys
+            | (1, 0) => neg ((neg xs) / ys)
+            | (0, 1) => neg (xs / (neg ys))
+            | (1, 1) => (neg xs) / (neg ys)
+
+def Bits.abs {n : ℕ} (xs : Bits n) : Bits n :=
+  if isNeg xs then neg xs else xs
+
+def Bits.smod {n : ℕ} (xs ys : Bits n) : Bits n :=
+  if ys = 0
+  then 0
+  else let mod := (abs xs) % (abs ys)
+       if isNeg xs then neg mod else mod
+
+
+def Bool.toBits {k} : Bool → Bits k
+  | .false => 0
+  | .true => 1
+
+def Bools.toBits : ∀ n, List Bool → Bits n
+  | 0, _ => ⦃⦄
+  | n + 1, [] => 0 +> toBits n []
+  | n + 1, x :: xs => x +> toBits n xs
+
+def Nat.toBitsAux' (n : Nat) : List Bool :=
+  if n < 2
+  then [n.toBool]
+  else (n % 2).toBool :: (n / 2).toBitsAux'
+
+def Nat.toBits' (m n : Nat) : Bits m :=
+  let bs := (List.takeD m (Nat.toBitsAux' n) 0).reverse
+  Bools.toBits m bs
+
+def Bits.addmod {n : ℕ} (x y z : Bits n) : Bits n :=
+  if z = 0
+  then 0
+  else Nat.toBits' n ((x.toNat + y.toNat) % z.toNat) -- (x + y) % z
+
+def Bits.mulmod {n : ℕ} (x y z : Bits n) : Bits n :=
+  if z = 0
+  then 0
+  else Nat.toBits' n ((x.toNat * y.toNat) % z.toNat) -- (x + y) % z
+
+def Bits.expNat {n : ℕ} (x : Bits n) : Nat → Bits n
+  | 0 => 1
+  | k + 1 => x * x.expNat k
+
+def Bits.exp {n : ℕ} (x y : Bits n) : Bits n := expNat x y.toNat
+
+instance {n} : HPow (Bits n) (Bits n) (Bits n) := ⟨Bits.exp⟩
+
+inductive Bits.Signext : Nat → Bool → ∀ {n}, Bits n → Bits n → Prop
+  | zero : ∀ n x (xs : Bits n), Signext 0 x (x +> xs) (x +> xs)
+  | succ :
+    ∀ m n x y (xs ys : Bits n),
+      Signext m y xs ys →
+      Signext (m + 1) y (x +> xs) (y +> ys)
+
+def Bits.prefix {m} : ∀ {n}, Bits (m + n) → Bits n
+  | 0, _ => ⦃⦄
+  | n + 1, x +> xs => x +> xs.prefix
+
+def Bits.suffix : ∀ {m n}, Bits (m + n) → Bits m
+  | _, 0, xs => xs
+  | _, n + 1, _ +> xs => xs.suffix
+
+theorem Bits.prefix_append {m n} (xs : Bits m) (ys : Bits n) :
+    (xs ++ ys).prefix = xs := by
+  induction m with
+  | zero => apply nil_eq_nil
+  | succ m ih =>
+    match xs with
+    | x +> xs => rw [cons_append]; simp [Bits.prefix, ih]
+
+theorem Bits.suffix_append {m n} (xs : Bits m) (ys : Bits n) :
+    (xs ++ ys).suffix = ys := by
+  induction m with
+  | zero => cases xs; rfl
+  | succ m ih =>
+    match xs with
+    | x +> xs => rw [cons_append]; simp [Bits.suffix, ih]
+
+theorem Bits.append_inj {m n} {xs₁ ys₁ : Bits m} {xs₂ ys₂ : Bits n} :
+     xs₁ ++ xs₂ = ys₁ ++ ys₂ → xs₁ = ys₁ ∧ xs₂ = ys₂ := by
+  induction m generalizing xs₂ ys₂ n with
+  | zero => cases xs₁; cases ys₁; intro h; refine' ⟨nil_eq_nil, h⟩
+  | succ n ih =>
+    match xs₁, ys₁ with
+    | x +> xs, y +> ys =>
+      simp [Bits.cons_append]; intro h h'
+      let ⟨ih₁, ih₂⟩ := ih h'
+      refine ⟨⟨h, ih₁⟩, ih₂⟩
+
+def Addr.toWord (a : Addr) : Bits 256 := (0 : Bits 96) ++ a
+
+theorem Addr.toWord_inj {a a' : Addr} :
+    Addr.toWord a = Addr.toWord a' → a = a' := And.right ∘ Bits.append_inj
+
+def Nat.toBits (k) : Nat → Bits k
+  | 0 => 0
+  | n + 1 => (Nat.toBits k n).succ
+
+theorem Bits.zero_eq_cons {n} : (0 : Bits (n + 1)) = 0 +> (0 : Bits n) := rfl
+theorem Bits.max_eq_cons {n} : max (n + 1) = 1 +> max n := rfl
+
+theorem Bits.eq_max_iff_isMax {k : ℕ} (xs : Bits k) : xs = max k ↔ xs.isMax = true := by
+  induction xs with
+  | nil => apply iff_of_true <;> rfl
+  | cons x xs ih =>
+    rw [max_eq_cons, cons_eq_cons, ih]
+    simp only [isMax, Bool.and_eq_true]; rfl
+
+theorem Bits.max_isMax {n : ℕ} : (max n).isMax = true := by
+  rw [← eq_max_iff_isMax]
+
+theorem Bits.succ_toNat_max_eq_pow {n : Nat} : (max n).toNat.succ = 2 ^ n := by
+  induction n with
+  | zero => rfl
+  | succ n ih =>
+    simp [max, toNat, Nat.two_pow_succ];
+    rw [← ih]; rfl
+
+theorem Bits.toNat_max_add_one_eq_pow {n : Nat} : (max n).toNat + 1 = 2 ^ n :=
+  succ_toNat_max_eq_pow
+
+theorem Bits.toNat_succ {k : ℕ} (xs : Bits k) :
+    xs.succ.toNat = cond xs.isMax 0 xs.toNat.succ := by
+  induction xs with
+  | nil => rfl
+  | cons x xs ih =>
+    by_cases h : xs = max _
+    · have h' := (eq_max_iff_isMax xs).mp h
+      simp [h'] at ih; simp only [succ, isMax, toNat, h', ih]
+      cases x <;> simp; rw [← succ_toNat_max_eq_pow, h]
+    · have h' := mt (eq_max_iff_isMax xs).mpr h
+      simp [h'] at ih
+      simp only [succ, toNat, isMax, h']
+      rw [← Nat.add_succ]; simp [ih]
+
+instance {m n} : OfNat (Bits m) n := ⟨Nat.toBits _ n⟩
+
+def Nat.toByte : Nat → Bits 8 := Nat.toBits _
+
+def toAddr : Bits 256 → Bits 160 := @Bits.suffix 160 96
+
+def suffix_append {m n} {xs : Bits m} {ys : Bits n} :
+    Bits.suffix (xs ++ ys) = ys := by
+  induction m with
+  | zero => cases xs; rfl
+  | succ m ih =>
+    match xs with
+    | x +> xs' =>
+      simp [Bits.cons_append, Bits.suffix];
+      apply ih
+
+theorem toAddr_toWord (a : Addr) : toAddr (Addr.toWord a) = a := suffix_append
+
+theorem Bits.prefix_append_suffix {m n} :
+    ∀ xs : Bits (m + n), xs.prefix ++ xs.suffix = xs := by
+  induction n with
+  | zero => intro xs; rfl
+  | succ n ih =>
+    intro xs; match xs with
+    | x +> xs' => simp [Bits.prefix, suffix, cons_append, ih]
+
+def Bits.toBytes : ∀ {n}, Bits (8 * n) → Bytes
+  | 0, ⦃⦄ => []
+  | _ + 1, b0 +> b1 +> b2 +> b3 +> b4 +> b5 +> b6 +> b7 +> bs =>
+    ⦃b0, b1, b2, b3, b4, b5, b6, b7⦄ :: bs.toBytes
+
+abbrev Nib : Type := Bits 4
+
+def Bytes.toBits' : ∀ (n : Nat), Bytes → Bits (8 * n)
+  | 0, _ => ⦃⦄
+  | n + 1, [] => (0 : Byte) ++ toBits' n []
+  | n + 1, b :: bs => b ++ toBits' n bs
+
+def Bytes.toBits (n : Nat) (bs : Bytes) : Bits (8 * n) :=
+  Bytes.toBits' n <| List.reverse <| List.takeD n (List.reverse bs) 0
+
+theorem Bits.cons_eq_zero_iff {n x} {xs : Bits n} :
+   x +> xs = 0 ↔ (x = 0 ∧ xs = 0) := by rw [zero_eq_cons]; simp
+
+theorem Bits.zero_append_zero {m n} :
+    (0 : Bits n) ++ (0 : Bits m) = (0 : Bits (m + n)) := by
+  induction n with
+  | zero => rfl
+  | succ n ih => rw [zero_eq_cons, zero_eq_cons, cons_append, ih]
+
+theorem Bits.toNat_zero : ∀ {k}, (0 : Bits k).toNat = 0
+  | 0 => rfl
+  | k + 1 => by rw [zero_eq_cons]; simp [toNat, @toNat_zero k]; rfl
+
+theorem Bits.sub_add_cancel : ∀ {n} {x y : Bits n}, x - y + y = x := by
+  apply rec2; rfl
+  intro n x xs y ys ih
+  rw [cons_sub_cons, cons_add_cons, ih]
+  apply congr_arg₂ _ _ rfl
+  rw [← Bits.faux]; cases (lt' xs ys) <;> cases y <;> simp
+
+theorem Bits.add_left_inj {n} :
+    ∀ {xs ys zs : Bits n}, xs + ys = xs + zs → ys = zs := by
+  induction n with
+  | zero => intro _ _ _ _; apply nil_eq_nil
+  | succ n ih =>
+    intro xs ys zs h
+    match xs, ys, zs with
+    | x +> xs, y +> ys, z +> zs =>
+      simp [cons_add_cons] at h
+      simp [ih h.right] at *; assumption
+
+theorem Bits.toNat_lt_pow {n} (xs : Bits n) : xs.toNat < 2 ^ n := by
+  induction xs with
+  | nil => simp [toNat]
+  | cons x xs ih =>
+    simp only [toNat]; rw [Nat.two_pow_succ]
+    apply Nat.add_lt_add_of_le_of_lt _ <| ih
+    cases x <;> simp
+
+theorem Bits.toNat_inj :
+    ∀ {k} (xs ys : Bits k), xs.toNat = ys.toNat → xs = ys := by
+  apply rec2
+  · intro _; rfl
+  · intro n x xs y ys ih h; simp only [toNat] at h
+    cases x <;> cases y <;> simp at h <;> try {rw [ih h]}
+    · apply (Nat.ne_of_lt (lt_of_lt_of_le (toNat_lt_pow _) _) h).elim
+      apply Nat.le_add_right
+    · apply (Nat.ne_of_lt (lt_of_lt_of_le (toNat_lt_pow _) _) h.symm).elim
+      apply Nat.le_add_right
+
+theorem Bits.eq_max_iff_succ_toNat_eq_pow {n : Nat} (xs : Bits n) :
+     xs = max _ ↔ xs.toNat.succ = 2 ^ n := by
+  constructor <;> intro h
+  · rw [h]; apply succ_toNat_max_eq_pow
+  · apply toNat_inj; rw [← Nat.succ_inj, succ_toNat_max_eq_pow, h]
+
+theorem toNat_toBits {k n} (h : n < 2 ^ k) : (Nat.toBits k n).toNat = n := by
+  induction n with
+  | zero => simp [Nat.toBits, Bits.toNat_zero]
+  | succ n ih =>
+    simp only [Nat.toBits]
+    rw [Bits.toNat_succ]
+    have ih' := ih <| lt_trans (Nat.lt_succ_self n) h
+    by_cases h' : Nat.toBits k n = Bits.max k
+    · have h_eq := @Bits.succ_toNat_max_eq_pow k
+      rw [← h', ih'] at h_eq; rw [← h_eq] at h; cases Nat.lt_irrefl _ h
+    · simp [mt (Bits.eq_max_iff_isMax (Nat.toBits k n)).mpr h', ih']
+
+theorem Nat.toBits_inj {k m n : ℕ} (hm : m < 2 ^ k) (hn : n < 2 ^ k)
+    (h : toBits k m = toBits k n) : m = n := by
+  rw [← toNat_toBits hm, ← toNat_toBits hn, h]
+
+theorem Bits.nil_le_nil {xs ys : Bits 0} : xs ≤ ys := by
+  cases xs; cases ys; constructor
+
+theorem Bits.lt_succ_self {n} {xs : Bits n} (h : xs ≠ max n) : xs < xs.succ := by
+  induction xs with
+  | nil => cases (h nil_eq_nil)
+  | cons x xs ih =>
+    simp only [Ne, max_eq_cons, cons_eq_cons] at h
+    cases x <;> simp [succ]
+    · by_cases h' : xs = max _
+      · left; simp [h', max_isMax]
+      · right;
+        simp [mt (eq_max_iff_isMax xs).mpr h']
+        apply ih h'
+    · simp [Bool.one] at h;
+      simp [mt (eq_max_iff_isMax xs).mpr h]
+      right; simp; apply ih h
+
+theorem Bits.lt_trans {n} {xs ys zs : Bits n} (h : xs < ys) (h' : ys < zs) : xs < zs := by
+  induction n with
+  | zero => cases xs; cases ys; cases h
+  | succ n ih =>
+    match xs, ys, zs with
+    | x +> xs, y +> ys, z +> zs =>
+      rcases h with h | ⟨⟨_⟩, h⟩ <;> rcases h' with h' | ⟨⟨_⟩, h'⟩
+      · left; apply Bool.lt_trans h h'
+      · left; apply h
+      · left; apply h'
+      · right; refine ⟨rfl, ih h h'⟩
+
+theorem Bits.le_refl {n} {xs : Bits n} : xs ≤ xs := by
+  induction xs with
+  | nil => apply nil_le_nil
+  | cons x xs ih => simp [cons_le_cons]; exact ih
+
+theorem Bits.le_of_lt {n : Nat} {xs ys : Bits n} (h : xs < ys) : xs ≤ ys := by
+  induction n with
+  | zero => cases xs; cases ys; cases h
+  | succ n ih =>
+    match xs, ys with
+    | x +> xs, y +> ys =>
+      rw [cons_lt_cons] at h
+      rcases h with h | ⟨h, h'⟩
+      · left; exact h
+      · right; refine ⟨h, ih h'⟩
+
+theorem Bits.lt_or_eq_of_le {n : Nat} {xs ys : Bits n} (h : xs ≤ ys) :
+    xs < ys ∨ xs = ys := by
+  induction n with
+  | zero => cases xs; cases ys; simp
+  | succ n ih =>
+    match xs, ys with
+    | x +> xs, y +> ys =>
+      rcases h with h | ⟨⟨_⟩, h⟩
+      · left; left; exact h
+      · rcases ih h with h | ⟨⟨_⟩⟩
+        · left; right; refine ⟨rfl, h⟩
+        · right; rfl
+
+theorem Bits.zero_le {n} : ∀ xs : Bits n, 0 ≤ xs := by
+  induction n with
+  | zero => intro xs; cases xs; constructor
+  | succ n ih =>
+    intro xs; match xs with
+    | x +> xs =>
+      rw [zero_eq_cons, cons_le_cons]
+      cases x
+      · right; refine ⟨rfl, ih xs⟩
+      · left; constructor
+
+theorem Bits.lt_of_le_of_lt {n} {xs ys zs : Bits n}
+    (h : xs ≤ ys) (h' : ys < zs) : xs < zs := by
+  cases lt_or_eq_of_le h with
+  | inl h'' => apply lt_trans h'' h'
+  | inr h'' => rw [h'']; exact h'
+
+theorem Bits.le_of_le_of_lt {n} {xs ys zs : Bits n}
+    (h : xs ≤ ys) (h' : ys < zs) : xs ≤ zs :=
+  le_of_lt <| lt_of_le_of_lt h h'
+
+theorem Nat.toBits_le_toBits {k m n : Nat} (h_le : m ≤ n) (h_lt : n < 2 ^ k) :
+    (@toBits k m) ≤ (@toBits k n) := by
+  induction n generalizing m with
+  | zero => rw [le_zero] at h_le; cases h_le; apply Bits.zero_le
+  | succ n ih =>
+    rw [le_add_one_iff] at h_le
+    rcases h_le with h_le | h_eq
+    · have h_lt' := lt_trans (lt_succ_self n) h_lt
+      have hh := ih h_le h_lt'
+      simp [toBits]
+      apply Bits.le_of_le_of_lt hh _
+      apply Bits.lt_succ_self
+      intro hc;
+      rw [Bits.eq_max_iff_succ_toNat_eq_pow, toNat_toBits h_lt'] at hc
+      rw [← hc] at h_lt; cases Nat.lt_irrefl _ h_lt
+    · rw [h_eq]; apply Bits.le_refl
+
+def Nib.toHexit : Nib → Char
+  | ⦃0, 0, 0, 0⦄ => '0'
+  | ⦃0, 0, 0, 1⦄ => '1'
+  | ⦃0, 0, 1, 0⦄ => '2'
+  | ⦃0, 0, 1, 1⦄ => '3'
+  | ⦃0, 1, 0, 0⦄ => '4'
+  | ⦃0, 1, 0, 1⦄ => '5'
+  | ⦃0, 1, 1, 0⦄ => '6'
+  | ⦃0, 1, 1, 1⦄ => '7'
+  | ⦃1, 0, 0, 0⦄ => '8'
+  | ⦃1, 0, 0, 1⦄ => '9'
+  | ⦃1, 0, 1, 0⦄ => 'A'
+  | ⦃1, 0, 1, 1⦄ => 'B'
+  | ⦃1, 1, 0, 0⦄ => 'C'
+  | ⦃1, 1, 0, 1⦄ => 'D'
+  | ⦃1, 1, 1, 0⦄ => 'E'
+  | ⦃1, 1, 1, 1⦄ => 'F'
+
+def Byte.nib0 : Byte → Nib
+  | ⦃w, x, y, z, _, _, _, _⦄ => ⦃w, x, y, z⦄
+
+def Byte.nib1 : Byte → Nib
+  | ⦃_, _, _, _, w, x, y, z⦄ => ⦃w, x, y, z⦄
+
+def Byte.toHex (b : Byte) : String :=
+⟨[b.nib0.toHexit, b.nib1.toHexit]⟩
+
+def Bytes.toString : Bytes → String
+  | [] => ""
+  | [b] => b.toString
+  | b :: bs => b.toString ++ " " ++ toString bs
+
+instance : Repr Bytes := ⟨λ b _ => b.toString⟩
+
+def Ox (hx hx' : Nib) : Byte := hx ++ hx'
+
+theorem nib0_eq : ∀ {x y : Nib}, (Ox x y).nib0 = x
+| ⦃_, _, _, _⦄, ⦃_, _, _, _⦄ => rfl
+
+def x0 : Nib := ⦃0, 0, 0, 0⦄
+def x1 : Nib := ⦃0, 0, 0, 1⦄
+def x2 : Nib := ⦃0, 0, 1, 0⦄
+def x3 : Nib := ⦃0, 0, 1, 1⦄
+def x4 : Nib := ⦃0, 1, 0, 0⦄
+def x5 : Nib := ⦃0, 1, 0, 1⦄
+def x6 : Nib := ⦃0, 1, 1, 0⦄
+def x7 : Nib := ⦃0, 1, 1, 1⦄
+def x8 : Nib := ⦃1, 0, 0, 0⦄
+def x9 : Nib := ⦃1, 0, 0, 1⦄
+def xA : Nib := ⦃1, 0, 1, 0⦄
+def xB : Nib := ⦃1, 0, 1, 1⦄
+def xC : Nib := ⦃1, 1, 0, 0⦄
+def xD : Nib := ⦃1, 1, 0, 1⦄
+def xE : Nib := ⦃1, 1, 1, 0⦄
+def xF : Nib := ⦃1, 1, 1, 1⦄
+
+def Bytes.sig (bs : Bytes) : Bytes :=
+  List.dropWhile (· = 0) bs
+
+theorem Bool.lt_or_ge (x y : Bool) : x < y ∨ x ≥ y := by
+  cases x <;> cases y <;> simp
+
+theorem Bool.lt_or_eq_of_le {x y : Bool} : x ≤ y → (x < y ∨ x = y) := by
+  cases x <;> cases y <;> simp
+
+theorem Bits.lt_or_ge {n : ℕ} : ∀ xs ys : Bits n, xs < ys ∨ xs ≥ ys := by
+  induction n with
+  | zero =>
+    intros xs ys; cases xs; cases ys
+    right; constructor
+  | succ n ih =>
+    intros xs ys
+    match xs, ys with
+    | x +> xs, y +> ys =>
+      rcases Bool.lt_or_ge x y with h | h
+      · left; left; exact h
+      · rcases Bool.lt_or_eq_of_le h  with h' | h'
+        · right; left; exact h'
+        · rcases ih xs ys with h'' | h''
+          · left; right; refine ⟨h'.symm, h''⟩
+          · right; right; refine ⟨h', h''⟩
+
+theorem Bits.not_lt {n : ℕ} (xs ys : Bits n) : ¬ xs < ys ↔ ys ≤ xs := by
+  constructor
+  · rw [← or_iff_not_imp_left]; apply lt_or_ge
+  · intros h h'; cases lt_irrefl <| lt_of_le_of_lt h h'
+
+theorem overflow_iff_overflow_eq_true :
+    ∀ {n : ℕ} (xs ys : Bits n), Overflow xs ys ↔ overflow xs ys = true := by
+  apply @Bits.rec2 (λ n xs ys => Overflow xs ys ↔ overflow xs ys = true)
+  · apply iff_of_false
+    · simp [Overflow]; rfl
+    · simp [overflow]
+  · intro n x xs y ys ih
+    simp only [Overflow, Bits.toNat, overflow, Nat.two_pow_succ]
+    cases x <;> cases y <;> simp
+    · apply Nat.add_lt_add <;> apply Bits.toNat_lt_pow
+    · rw [← ih, Nat.add_comm _ ys.toNat]
+      rw [← Nat.add_assoc, Nat.add_le_add_iff_right]
+      simp [Overflow]
+    · rw [Nat.add_assoc, Nat.add_le_add_iff_left, ← ih]
+      simp [Overflow]
+    · omega
+
+theorem Bits.toNat_lt_toNat :
+    ∀ {k} (xs ys : Bits k), xs < ys → xs.toNat < ys.toNat := by
+  apply rec2
+  · intro h; cases h
+  · intro k x xs y ys ih h
+    rcases h with h | h
+    · rw [Bool.lt_iff] at h; rcases h with ⟨⟨_⟩, ⟨_⟩⟩;simp [toNat]
+      apply le_trans (toNat_lt_pow xs) <| Nat.le_add_right _ _
+    · rcases h with ⟨⟨_⟩, h⟩; simp [toNat]; apply ih h
+
+theorem Bits.toNat_le_toNat {k} (xs ys : Bits k) (h : xs ≤ ys) :
+    xs.toNat ≤ ys.toNat := by
+  rcases lt_or_eq_of_le h with h | ⟨⟨_⟩⟩
+  · apply Nat.le_of_lt <| toNat_lt_toNat _ _ h
+  · apply Nat.le_refl
+
+theorem Bool.beq_eq_true (a b : Bool) : ((a == b) = true) = (a = b) := by
+  cases a <;> cases b <;> simp
+
+theorem Bits.lt_iff_lt' {k} (xs ys : Bits k) :
+    xs < ys ↔ lt' xs ys = true := by
+  induction k with
+  | zero =>
+    cases xs; cases ys
+    apply iff_of_false <;> {intro h; cases h}
+  | succ k ih =>
+    match xs, ys with
+    | x +> xs, y +> ys =>
+     simp only [lt']
+     rw [cons_lt_cons, Bool.or_eq_true, Bool.and_eq_true (_ == _)]
+     rw [← ih, Bool.beq_eq_true]; simp only [LT.lt]
+
+theorem Bits.sub_self {n} {xs : Bits n} : xs - xs = 0 := by
+  induction xs with
+  | nil => rfl
+  | cons x xs ih =>
+    rw [cons_sub_cons]; cases x <;>
+    simp [ih, mt (lt_iff_lt' _ _).mpr <| @Bits.lt_irrefl _ xs] <;> rfl
+
+theorem Bits.toNat_add {k} (xs ys : Bits k) :
+    (xs + ys).toNat = xs.toNat + ys.toNat - (cond (overflow xs ys) (2 ^ k) 0) := by
+  apply @Bits.rec2
+    (λ k xs ys => (xs + ys).toNat = xs.toNat + ys.toNat - (cond (overflow xs ys) (2 ^ k) 0))
+  · simp [toNat, @eq_nil (⦃⦄ + ⦃⦄)]
+  · intro k x xs y ys ih
+    rw [cons_add_cons]; simp only [overflow, toNat]; rw [ih]
+    rcases Bool.eq_false_or_eq_true (overflow xs ys) with h'' | h'' <;>
+      rw [h''] <;> cases x <;> cases y <;> simp <;>
+      try {rw [Nat.two_pow_succ]} <;> try {omega}
+    · rw [← Nat.add_sub_assoc, Nat.add_sub_cancel_left]
+      rw [← overflow_iff_overflow_eq_true] at h''; exact h''
+    · have h_rw : 2 ^ k + xs.toNat + (2 ^ k + ys.toNat) =
+                    xs.toNat + ys.toNat + (2 ^ k + 2 ^ k) := by omega
+      rw [← Nat.add_sub_assoc, Nat.add_sub_cancel_left, h_rw]; omega
+      rw [← overflow_iff_overflow_eq_true] at h''; exact h''
+
+theorem Bits.toNat_add_eq_of_nof {k} (xs ys : Bits k) (h : Nof xs ys) :
+    (xs + ys).toNat = xs.toNat + ys.toNat := by
+  rw [nof_iff_not_overflow, overflow_iff_overflow_eq_true] at h
+  rw [toNat_add]; simp [h]
+
+theorem Bits.toNat_sub {k} (xs ys : Bits k) :
+    (xs - ys).toNat = (cond (lt' xs ys) (2 ^ k) 0) + xs.toNat - ys.toNat := by
+  induction k with
+  | zero => cases xs; cases ys; simp [lt', @eq_nil (⦃⦄ - ⦃⦄), toNat]
+  | succ k ih =>
+    match xs, ys with
+    | x +> xs, y +> ys =>
+      have h : ys.toNat ≤ 2 ^ k + xs.toNat :=
+        le_trans (Nat.le_of_lt <| toNat_lt_pow _) <| Nat.le_add_right _ _
+      have h' : lt' xs ys = false → ys.toNat ≤ xs.toNat := by
+        intro h; apply toNat_le_toNat; rw [← not_lt, lt_iff_lt', h]; simp
+      rw [cons_sub_cons]; simp only [toNat, lt']; rw [ih]
+      rcases Bool.eq_false_or_eq_true (lt' xs ys) with h'' | h'' <;>
+        rw [h''] <;> cases x <;> cases y <;> simp <;> try rw [Nat.two_pow_succ]
+      · rw [← Nat.add_sub_assoc h, Nat.add_assoc]
+      · omega
+      · rw [Nat.sub_add_eq, ← Nat.add_sub_assoc h]; omega
+      · rw [Nat.sub_add_eq, ← Nat.add_sub_assoc (h' h'')]; omega
+      · rw [Nat.add_sub_assoc (h' h'')]
+      · rw [Nat.sub_add_eq, Nat.add_sub_cancel_left]
+
+theorem Bits.toNat_sub_eq_of_le {k} (xs ys : Bits k) (h : ys ≤ xs) :
+    (xs - ys).toNat = xs.toNat - ys.toNat := by
+  rw [toNat_sub]; rw [← not_lt, lt_iff_lt'] at h; simp [h]
+
+theorem Bits.append_eq_append_iff {m n} {xs ys : Bits m} {xs' ys' : Bits n} :
+    xs ++ xs' = ys ++ ys' ↔ (xs = ys ∧ xs' = ys') := by
+  revert xs xs' ys ys' n
+  induction m with
+  | zero =>
+    intros n xs ys xs' ys'
+    cases xs; cases ys; simp; rfl
+  | succ m ih =>
+    intros n xs ys xs' ys'
+    rcases xs with _ | ⟨x, xs⟩
+    rcases ys with _ | ⟨y, ys⟩
+    simp [Bits.cons_append]
+    rw [ih]; simp [and_assoc]
+
+theorem Bits.length_toBytes {n} (xs : Bits (8 * n)) : xs.toBytes.length = n := by
+  induction n with
+  | zero => cases xs; rfl
+  | succ n ih =>
+    match xs with
+    | _ +> _ +> _ +> _ +> _ +> _ +> _ +> _ +> _ =>
+      simp [toBytes]; apply ih
+
+theorem toBits'_toBytes {n} (xs : Bits (8 * n)) :
+    Bytes.toBits' n (Bits.toBytes xs) = xs := by
+  induction n with
+  | zero => cases xs; rfl
+  | succ n ih =>
+    match xs with
+    | _ +> _ +> _ +> _ +> _ +> _ +> _ +> _ +> xs' =>
+      simp only [Bits.toBytes, Bytes.toBits']; rw [ih]; rfl
+
+theorem toBits_toBytes {n} (xs : Bits (8 * n)) :
+    Bytes.toBits n (Bits.toBytes xs) = xs := by
+  simp only [Bytes.toBits];
+  rw [List.takeD_eq_self, List.reverse_reverse]
+  · apply toBits'_toBytes
+  · rw [List.length_reverse, Bits.length_toBytes]
+
+theorem Bits.succ_cons {n} (x) (xs : Bits n) :
+     (x +> xs).succ = (x != xs.isMax) +> xs.succ := rfl
+
+theorem Bits.append_eq_max_iff {m n} (xs : Bits m) (ys : Bits n) :
+    (xs ++ ys) = max (n + m) ↔ (xs = max m ∧ ys = max n) := by
+  induction xs with
+  | nil => simp [@nil_eq_nil ⦃⦄ (max 0)]; rfl
+  | cons x xs ih =>
+    rw [cons_append]; conv => lhs; rhs; apply (@max_eq_cons (n + _))
+    rw [cons_eq_cons, ih, max_eq_cons, cons_eq_cons, and_assoc]
+
+theorem Bits.max_append_max {m n} :
+    max m ++ max n = max (n + m) := by
+  induction m with
+  | zero => rfl
+  | succ m ih => simp [max]; rw [cons_append, ih]
+
+theorem Bits.succ_append {m n} (xs : Bits m) (ys : Bits n) :
+    (xs ++ ys).succ = (if ys = max n then xs.succ else xs) ++ ys.succ := by
+  induction xs with
+  | nil => split <;> rfl
+  | cons x xs ih =>
+    rename Nat => m
+    have h_rw : (xs = max m ∧ ys = max n) ↔ (xs ++ ys).isMax = true := by
+      rw [← append_eq_max_iff, eq_max_iff_isMax]
+    rw [cons_append]; simp only [succ_cons]; rw [ih]
+    by_cases h : xs = max _ <;> by_cases h' : ys = max n <;>
+      simp [h, h'] <;> simp [h, h'] at h_rw
+    · simp [h_rw, max_isMax, cons_append]
+    · simp [h_rw, cons_append]
+    · simp [h_rw, mt (eq_max_iff_isMax _).mpr h, cons_append]
+    · simp [h_rw, cons_append]
+
+theorem Bits.toBytes_eq_cons {n} (b : Byte) {xs : Bits (8 * n)} :
+    @toBytes (n + 1) (b ++ xs) = b :: toBytes xs := by
+  match b with
+  | ⦃_, _, _, _, _, _, _, _⦄ => rfl
+
+def Bits.factor {k m} : ∀ {n}, Bits (k * m + k * n) → Bits (k * (m + n))
+  | 0, xs => xs
+  | _ + 1, xs => xs.prefix.prefix ++ Bits.factor (xs.prefix.suffix ++ xs.suffix)
+
+def Bits.fappend {k m n} (xs : Bits (k * m)) (ys : Bits (k * n)) : Bits (k * (n + m)) :=
+  factor <| xs ++ ys
+
+def Bits.fappend_eq_append {k m n}
+    (xs : Bits (k * (m + 1))) (ys : Bits (k * n)) :
+    fappend xs ys = xs.prefix ++ fappend xs.suffix ys := by
+  simp [fappend, factor, prefix_append, suffix_append]
+
+theorem Bits.toBytes_eq_append {m n} {xs : Bits (8 * m)} {ys : Bits (8 * n)} :
+    toBytes (fappend xs ys) = toBytes xs ++ toBytes ys := by
+  induction m with
+  | zero => cases xs; rfl
+  | succ m ih =>
+    have h_rw := @Bits.prefix_append_suffix (8 * m) 8 xs
+    conv => rhs; lhs; arg 1; apply h_rw.symm
+    rw [fappend_eq_append, toBytes_eq_cons, ih, toBytes_eq_cons, List.cons_append]
+
+instance {ξ : Type u} {ρ : ξ → Prop} {xs : List ξ}
+    [d : ∀ x : ξ, Decidable (ρ x)] : Decidable (xs.Forall ρ) := by
+  induction xs with
+  | nil => apply instDecidableTrue
+  | cons x xs ih => simp; apply instDecidableAnd
+
+def Bytes.Max (bs : Bytes) : Prop := bs.Forall (· = .max 8)
+
+instance (bs : Bytes) : Decidable bs.Max := by
+  unfold Bytes.Max; infer_instance
+
+def Bytes.succ : Bytes → Bytes
+  | [] => []
+  | b :: bs => (if Max bs then b.succ else b) :: succ bs
+
+theorem List.takeD_concat {ξ : Type u} (n) (xs : List ξ) (y) :
+    takeD n (xs.concat y) y = takeD n xs y := by
+  induction xs generalizing n with
+  | nil =>
+    match n with
+    | 0 => rfl
+    | n + 1 => rfl
+  | cons x xs ih =>
+    match n with
+    | 0 => rfl
+    | n + 1 =>
+      simp only [List.concat, takeD, headD, tail]; rw [ih]
+
+theorem Bytes.toBits_zero_cons {n} {bs} :
+    toBits n (0 :: bs) = toBits n bs := by
+  unfold toBits; rw [List.reverse_cons', List.takeD_concat]
+
+theorem Bytes.sig_toBits {n} (bs : Bytes) : bs.sig.toBits n = bs.toBits n := by
+  induction bs with
+  | nil => rfl
+  | cons b bs ih =>
+    unfold sig
+    by_cases hb : b = 0
+    · cases hb; rw [List.dropWhile_cons_of_pos _]
+      · apply Eq.trans ih; rw [toBits_zero_cons]
+      · rw [decide_eq_true rfl]
+    · rw [List.dropWhile_cons_of_neg _]
+      rw [decide_eq_false hb]; simp
+
+theorem toBytes_zero_eq_replicate_zero {n} :
+    (@Bits.toBytes n 0) = List.replicate n (0 : Byte) := by
+  induction n with
+  | zero => rfl
+  | succ n ih =>
+    have h : (0 : Bits (8 * (n + 1))) = (0 : Byte) ++ (0 : Bits (8 * n)) := rfl
+    rw [h]; simp [Bits.toBytes_eq_cons, List.replicate, ih]
+
+theorem Bits.zero_ne_succ' {n} :
+    zero (n + 1) ≠ (zero (n + 1)).succ := by
+  induction n with
+  | zero => intro h; cases h
+  | succ n ih =>
+    have h_rw : zero (n + 2) = 0 +> (zero (n + 1)) := rfl
+    rw [h_rw, succ_cons]
+    intro hc; rw [cons_eq_cons] at hc
+    apply ih hc.right
+
+theorem Bits.zero_ne_succ {n} :
+    (0 : Bits (n + 1)) ≠ (0 : Bits (n + 1)).succ := zero_ne_succ'
+
+theorem Bits.add_comm {n} {xs ys : Bits n} : xs + ys = ys + xs := by
+  apply toNat_inj; simp [toNat_add]; rw [Nat.add_comm, overflow_comm]
+
+theorem Bits.invert_zero_eq_max {n} : ~ (0 : Bits n) = max _ := by
+  induction n with
+  | zero => apply nil_eq_nil
+  | succ n ih => rw [zero_eq_cons]; simp only [max, not]; rw [ih]; rfl
+
+theorem Bits.zipWith_comm (f : Bool → Bool → Bool)
+    (hf : ∀ x y, f x y = f y x) (n) :
+    ∀ x y : Bits n, zipWith f x y = zipWith f y x := by
+  induction n with
+  | zero => intro xs ys; apply nil_eq_nil
+  | succ n ih =>
+    intros xs ys
+    match xs, ys with
+    | x +> xs, y +> ys =>
+      simp [zipWith, ih xs ys, hf x y]
+
+theorem Bits.and_comm {n} : ∀ (x y : Bits n), and x y = and y x := by
+  apply zipWith_comm; apply Bool.and_comm
+
+theorem Bits.zero_and {n} {xs : Bits n} : and (0 : Bits n) xs = 0 := by
+  induction n with
+  | zero => apply nil_eq_nil
+  | succ n ih =>
+    cases xs with
+    | cons xs x =>
+      rw [zero_eq_cons, cons_and_cons, ih]
+      cases x <;> rfl
+
+theorem Bits.and_zero {n} {xs : Bits n} : and xs (0 : Bits n) = 0 := by
+  rw [and_comm, zero_and]
+
+theorem toBits_toNat {k : ℕ} {xs : Bits k} : Nat.toBits k (Bits.toNat xs) = xs := by
+  apply Bits.toNat_inj; rw [toNat_toBits (Bits.toNat_lt_pow _)]
+
+theorem Bits.of_toNat_le_toNat {k : ℕ} {xs ys : Bits k}
+    (h : xs.toNat ≤ ys.toNat) : xs ≤ ys := by
+  have h' := Nat.toBits_le_toBits h (toNat_lt_pow _)
+  rw [toBits_toNat, toBits_toNat] at h'; exact h'
+
+theorem Bits.le_add_right {n} {xs ys : Bits n} (h : Nof xs ys) : xs ≤ xs + ys := by
+  apply of_toNat_le_toNat; rw [toNat_add_eq_of_nof _ _ h]; apply Nat.le_add_right
+
+def Hexit.toNib : Char → Option Nib
+  | '0' => some x0
+  | '1' => some x1
+  | '2' => some x2
+  | '3' => some x3
+  | '4' => some x4
+  | '5' => some x5
+  | '6' => some x6
+  | '7' => some x7
+  | '8' => some x8
+  | '9' => some x9
+  | 'a' => some xA
+  | 'b' => some xB
+  | 'c' => some xC
+  | 'd' => some xD
+  | 'e' => some xE
+  | 'f' => some xF
+  | 'A' => some xA
+  | 'B' => some xB
+  | 'C' => some xC
+  | 'D' => some xD
+  | 'E' => some xE
+  | 'F' => some xF
+  |  _  => none
+
+def Hex.toBits : ∀ (n : Nat), String → Option (Bits (4 * n))
+  | 0, ⟨[]⟩ => some ⦃⦄
+  | 0, ⟨_ :: _⟩ => none
+  | _ + 1, ⟨[]⟩ => none
+  | n + 1, ⟨c :: cs⟩ => do
+    let h ← Hexit.toNib c
+    let hs ← toBits n ⟨cs⟩
+    some (h ++ hs)
+
+def Char.toByte (c : Char) : Byte := Nat.toByte c.toNat
+def String.toBytes (s : String) : Bytes := s.data.map Char.toByte
+
+#eval String.toBytes "A1"
+
+def Bytes.toHex (bs : Bytes) : String :=
+  List.foldr (λ b s => Byte.toHex b ++ s) "" bs
+
+def Bits.toHex : ∀ k : Nat, Bits (4 * k) → String
+ | 0, ⦃⦄ => ""
+ | k + 1, .cons b0 (.cons b1 (.cons b2 (.cons b3 bs))) =>
+   ⟨[Nib.toHexit ⦃b0, b1, b2, b3⦄]⟩ ++ bs.toHex k
+
+def Byte.toB8 (b : Byte) : B8 := ⟨⟨b.toNat, b.toNat_lt_pow⟩⟩
+def Bits.toB64 (xs : Bits 64) : B64 := ⟨⟨xs.toNat, xs.toNat_lt_pow⟩⟩
+def B64.toBits (i : B64) : Bits 64 := Nat.toBits' 64 i.toBitVec.toFin.val
+
+def Bits.toB128 (xys : Bits 128) : B128 :=
+  let xs := @Bits.prefix 64 64 xys
+  let ys := @Bits.suffix 64 64 xys
+  ⟨xs.toB64, ys.toB64⟩
+
+def Bits.toB256 (xys : Bits 256) : B256 :=
+  let xs := @Bits.prefix 128 128 xys
+  let ys := @Bits.suffix 128 128 xys
+  ⟨xs.toB128, ys.toB128⟩
+
+def B128.toBits (i : B128) : Bits 128 := i.1.toBits ++ i.2.toBits
+def B256.toBits (i : B256) : Bits 256 := i.1.toBits ++ i.2.toBits
+
+def Bits.bexpCore : ∀ {m n : Nat}, Bits m → Bits n → (Bits m × Bits m)
+  | _, 0, _, ⦃⦄ => ⟨1, 1⟩
+  | _, 1, x, ⦃b⦄ => ⟨cond b x 1, x⟩
+  | m, n + 1, x, Bits.cons y ys =>
+    let ⟨r, s⟩ := @Bits.bexpCore m n x ys
+    let s₂ := s * s
+    ⟨(cond y s₂ 1) * r, s₂⟩
+
+def Bits.bexp {m : Nat} (xs ys : Bits m) : Bits m :=
+  (@Bits.bexpCore m m xs ys).fst
+
+instance : HPow B256 B256 B256 := ⟨B256.bexp⟩
+
+def Bits.ordering {n} (xs ys : Bits n) : Ordering :=
+  if xs < ys
+  then .lt
+  else if xs = ys
+       then .eq
+       else .gt
+
+instance {n} : Ord (Bits n) := ⟨Bits.ordering⟩
+
+instance {n} : XorOp (Bits n) := ⟨Bits.xor⟩
+
+instance {n : Nat} : ToString (Bits n) := ⟨@Bits.toString n⟩
+
+def Bytes.toNat (bs : Bytes) : Nat := --bs.toNat' 0
+  let rec aux (acc : Nat) : Bytes → Nat
+    | [] => acc
+    | b :: bs => aux ((acc * 256) + b.toNat) bs
+  aux 0 bs
+
+def Nat.toBytes : Nat → Bytes :=
+  let rec aux (n : Nat) : Bytes :=
+    if n < 256
+    then [n.toByte]
+    else (n % 256).toByte :: aux (n / 256)
+  List.reverse ∘ aux
+
+instance slt_decidable {n} (xs ys : Bits n) : Decidable (xs ±< ys) := by
+  induction n with
+  | zero => cases xs; cases ys; apply instDecidableFalse
+  | succ n ih =>
+    cases n with
+    | zero =>
+      match xs, ys with
+      | ⦃x⦄, ⦃y⦄ =>
+        rw [Bits.singleton_slt_singleton]
+        apply instDecidableAnd
+    | succ m =>
+      match xs, ys with
+      | xs +> x, ys +> y =>
+      apply instDecidableOr
+
+instance {n} (xs ys : Bits n) : Decidable (xs ±> ys) := by
+  unfold Bits.Sgt; apply slt_decidable
+
+-------------------------------- RLP --------------------------------
+
+
+inductive RLP : Type
+  | bytes : Bytes → RLP
+  | list : List RLP → RLP
+
+mutual def RLP.decode' : Nat → Bytes → Option (RLP × Bytes)
+    | _, [] => none
+    | 0, _ :: _ => none
+    | _ + 1, b@⦃0, _, _, _, _, _, _, _⦄ :: bs => some (.bytes [b], bs)
+    | _ + 1, b@⦃1, 0, 1, 1, 1, _, _, _⦄ :: bs => do
+      let (lbs, bs') ← List.splitAt? (b - Ox xB x7).toNat bs
+      let (rbs, bs'') ← List.splitAt? (Bytes.toNat lbs) bs'
+      return ⟨.bytes rbs, bs''⟩
+    | _ + 1, b@⦃1, 0, _, _, _, _, _, _⦄ :: bs =>
+      .map .bytes id <$> List.splitAt? (b - Ox x8 x0).toNat bs
+    | k + 1, b@⦃1, 1, 1, 1, 1, _, _, _⦄ :: bs => do
+      let (lbs, bs') ← List.splitAt? (b - Ox xF x7).toNat bs
+      let (rbs, bs'') ← List.splitAt? (Bytes.toNat lbs) bs'
+      let rs ← RLPs.decode k rbs
+      return ⟨.list rs, bs''⟩
+    | k + 1, b@⦃1, 1, _, _, _, _, _, _⦄ :: bs => do
+      let (rbs, bs') ← List.splitAt? (b - Ox xC x0).toNat bs
+      let rs ← RLPs.decode k rbs
+      return ⟨.list rs, bs'⟩
+  def RLPs.decode : Nat → Bytes → Option (List RLP)
+    | _, [] => some []
+    | 0, _ :: _ => none
+    | k + 1, bs@(_ :: _) => do
+      let (r, bs') ← RLP.decode' (k + 1) bs
+      let rs ← RLPs.decode k bs'
+      return (r :: rs)
+end
+
+def RLP.decode (bs : Bytes) : Option RLP :=
+  match RLP.decode' bs.length bs with
+  | some (r, []) => some r
+  | _ => none
+
+def RLP.encodeBytes : Bytes → Bytes
+  | [b] =>
+    if b < (Ox x8 x0)
+    then [b]
+    else [Ox x8 x1, b]
+  | bs =>
+    if bs.length < 56
+    then (Ox x8 x0 + bs.length.toByte) :: bs
+    else let lbs : Bytes := bs.length.toBytes
+         (Ox xB x7 + lbs.length.toByte) :: (lbs ++ bs)
+
+mutual
+  def RLP.encode : RLP → Bytes
+    | .bytes [b] =>
+      if b < (Ox x8 x0)
+      then [b]
+      else [Ox x8 x1, b]
+    | .bytes bs =>
+      if bs.length < 56
+      then (Ox x8 x0 + bs.length.toByte) :: bs
+      else let lbs : Bytes := bs.length.toBytes
+           (Ox xB x7 + lbs.length.toByte) :: (lbs ++ bs)
+    | .list rs => RLPs.encode rs
+  def RLPs.encodeMap : List RLP → Bytes
+    | .nil => []
+    | .cons r rs => r.encode ++ RLPs.encodeMap rs
+  def RLPs.encode (rs : List RLP) : Bytes :=
+    let bs := RLPs.encodeMap rs
+    let len := bs.length
+    if len < 56
+    then (Ox xC x0 + len.toByte) :: bs
+    else let lbs : Bytes := len.toBytes
+         (Ox xF x7 + lbs.length.toByte) :: (lbs ++ bs)
+end
+
+partial def RLP.toStrings : RLP → List String
+  | .bytes bs => [s!"0x{bs.toHex}"]
+  | .list rs => "List:" :: (rs.map RLP.toStrings).flatten.map ("  " ++ ·)
+
+lemma Bits._eq_zero (m n : Nat) :
+   ∀ (xs : Bits (m + n)),
+     Bits.and (Bits.max n ++ Bits.zero m) xs = 0 →
+     ∃ ys : Bits m, (Bits.zero n ++ ys) = xs := by
+  induction n with
+  | zero => intro xs _; refine' ⟨xs, rfl⟩
+  | succ n ih =>
+    intro xs h
+    match xs with
+    | x +> xs' =>
+      rw [max_eq_cons, cons_append, cons_and_cons, cons_eq_zero_iff] at h
+      simp [Bool.and] at h
+      rcases ih xs' h.right with ⟨ys, h'⟩
+      rw [← h', h.left]; refine' ⟨ys, rfl⟩
+
+-- the mask 0xffffffffffffffffffffffff0000000000000000000000000000000000000000,
+-- for checking that a given word is a valid Ethereum addresses
+def addressMask : Word := (@Bits.max 96) ++ (@Bits.zero 160)
+
+def Bits.toBools : ∀ {n}, Bits n → List Bool
+| 0, ⦃⦄ => []
+| _ + 1, x +> xs => x :: xs.toBools
+
+lemma Bits.toBools_inj :
+    ∀ {k : ℕ} (xs ys : Bits k), xs.toBools = ys.toBools → xs = ys := by
+  apply Bits.rec2
+  · intro _; rfl
+  · intro n x xs y ys ih h
+    simp [toBools] at h
+    rw [h.left, ih h.right]
+
+lemma Bits.toBools_append {m n : ℕ} (xs : Bits m) (ys : Bits n) :
+    (xs ++ ys).toBools = xs.toBools ++ ys.toBools := by
+  induction m with
+  | zero => cases xs; rfl
+  | succ m ih =>
+    cases xs; simp [cons_append, toBools]; apply ih
+
+lemma Bits.toBools_max {n : ℕ} : (max n).toBools = List.replicate n 1 := by
+  induction n with
+  | zero => rfl
+  | succ n ih => simp [max, toBools, List.replicate]; apply ih
+
+lemma Bits.toBools_zero {n : ℕ} : (zero n).toBools = List.replicate n 0 := by
+  induction n with
+  | zero => rfl
+  | succ n ih => simp [zero, toBools, List.replicate]; apply ih
+
+def Nat.toWord : Nat → Word := Nat.toBits 256
+def Nat.toWord' : Nat → Word := Nat.toBits' 256
+
+
+def Bools.shlo : List Bool → Bool → List Bool
+  | [], _ => []
+  | _ :: xs, x => xs ++ [x]
+
+def Bools.shl : Nat → List Bool → List Bool
+  | 0, xs => xs
+  | n + 1, xs => shlo (shl n xs) 0
+
+lemma Bits.toBools_snoc {n} (xs : Bits n) (y) :
+    (Bits.snoc xs y).toBools = xs.toBools ++ [y] := by
+  induction xs with
+  | nil => rfl
+  | cons x xs ih => simp [snoc, toBools, ih]
+
+lemma Bits.toBools_shlo {n} (xs : Bits n) (x) :
+    (Bits.shlo xs x).toBools = Bools.shlo xs.toBools x := by
+  cases xs; rfl; simp [shlo, toBools, Bools.shlo, toBools_snoc]
+
+lemma Bits.toBools_shl {m n} (xs : Bits n) :
+    (Bits.shl m xs).toBools = Bools.shl m xs.toBools := by
+  induction m generalizing xs with
+  | zero => rfl
+  | succ m ih => simp [shl, Bools.shl, toBools_shlo]; rw [ih]
+
+lemma Bits.max_append_zero {m n} :
+    Bits.max m ++ Bits.zero n = Bits.shl n (Bits.max (n + m)) := by
+  apply toBools_inj
+  rw [ toBools_append, toBools_zero, toBools_max,
+       toBools_shl, toBools_max, Nat.add_comm ]
+  induction n generalizing m with
+  | zero => simp [Bools.shl]
+  | succ n ih =>
+    simp [Bools.shl]
+    have h_rw : m + (n + 1) = m + 1 + n := by omega
+    rw [h_rw, ← ih]; simp [List.replicate, Bools.shlo]
+    apply List.replicate_add n 1 0
+
+lemma addressMask_eq_shl :
+    addressMask = Bits.shl (160 : Nat).toWord.toNat (Bits.max 256) := by
+  have h_rw : (160 : Nat).toWord.toNat = (160 : Nat) := by
+    apply toNat_toBits; omega
+  rw [h_rw]; apply Bits.max_append_zero
+
+lemma Bits.mask_and_eq_zero (m n : Nat) (xs : Bits (m + n))
+    (h : ∃ ys : Bits m, (Bits.zero n ++ ys) = xs) :
+    Bits.and (Bits.max n ++ Bits.zero m) xs = 0 := by
+  rcases h with ⟨a, h⟩
+  rw [← h, append_and_append, ← @zero_append_zero m n, append_eq_append_iff]
+  refine ⟨and_zero, zero_and⟩
+
+def comp {n} {ξ} (f : Bits (n + 1) → ξ) (x : Bool) (xs : Bits n) : ξ :=
+  f (x +> xs)
+
+@[irreducible] def sum : ∀ {m n}, (Bits m → Bits n) → Nat
+| 0, _, f => (f ⦃⦄).toNat
+| _ + 1, _, f => sum (comp f 0) + sum (comp f 1)
+
+lemma sum_zero {n} (f : Bits 0 → Bits n) : sum f = (f ⦃⦄).toNat := by delta sum; rfl
+
+lemma sum_succ {m n} (f : Bits (m + 1) → Bits n) :
+    sum f = sum (comp f 0) + sum (comp f 1) := by delta sum; rfl
+
+def SumNof {m n} (f : Bits m → Bits n) : Prop := sum f < 2 ^ n
+
+def Frel {A B} (a : A) (r : B → B → Prop) (f g : A → B) : Prop :=
+  ∀ a', (a = a' → r (f a') (g a')) ∧ (a ≠ a' → f a' = g a')
+
+lemma frel_succ {ξ} {n k b r} {f g : Bits (n + 1) → ξ} (h : Frel (b +> k) r f g) :
+    Frel k r (comp f b) (comp g b) ∧ (comp f !b) = (comp g !b) := by
+  constructor
+  · intro k'; constructor <;> intro h_k'
+    · apply (h (b +> k')).left (by rw [h_k'])
+    · apply (h (b +> k')).right
+      intro hc; rw [Bits.cons_eq_cons] at hc
+      cases h_k' hc.right
+  · apply funext; intro k'
+    apply (h ((!b) +> k')).right
+    intro hc; rw [Bits.cons_eq_cons] at hc
+    cases b <;> cases hc.left
+
+lemma sum_succ_with {m n} {f : Bits (m + 1) → Bits n} (b : Bool) :
+    sum f = sum (comp f b) + sum (comp f !b) := by
+  cases b; apply sum_succ; rw [Nat.add_comm (sum _)]; apply sum_succ
+
+lemma le_sum {m n} {f : Bits m → Bits n} {xs} : (f xs).toNat ≤ sum f := by
+  induction m with
+  | zero => rw [sum_zero]; cases xs; apply Nat.le_refl
+  | succ m ih =>
+    match xs with
+    | x +> xs =>
+      rw [sum_succ]
+      rcases Bool.zero_or_one x with h | h <;> cases h
+      · apply @le_trans _ _ _ (sum (comp f 0)) _ (@ih (comp f 0) xs) (Nat.le_add_right _ _)
+      · apply @le_trans _ _ _ (sum (comp f 1)) _ (@ih (comp f 1) xs) (Nat.le_add_left _ _)
+
+def Decrease {m n} (k : Bits m) (v : Bits n) (f g : Bits m → Bits n) : Prop :=
+  Frel k (λ x y => x - v = y) f g
+
+def Increase {m n} (k : Bits m) (v : Bits n) (f g : Bits m → Bits n) : Prop :=
+  Frel k (λ x y => x + v = y) f g
+
+open Bits
+
+lemma sum_sub_assoc {m n k v}
+    {f g : Bits m → Bits n}
+    (h : Decrease k v f g) (h' : v ≤ f k) :
+    sum f - v.toNat = sum g := by
+  induction m with
+  | zero =>
+    simp [sum_zero]; cases k
+    rw [← Bits.toNat_sub_eq_of_le _ _ h', (h ⦃⦄).left rfl]
+  | succ m ih =>
+    match k with
+    | b +> k =>
+      rcases frel_succ h with ⟨h_frel, h_eq⟩
+      rw [sum_succ_with b, sum_succ_with b, h_eq]
+      have h_le : toNat v ≤ sum (comp f b) := by
+        apply Nat.le_trans _ (@le_sum _ _ _ k)
+        apply toNat_le_toNat _ _ h'
+      conv =>
+        lhs;
+        rw [Nat.add_comm]
+        rw [Nat.add_sub_assoc h_le]
+        rw [ih h_frel h']
+        rw [Nat.add_comm ]
+        rfl
+
+lemma sum_add_assoc {m n k v} {f g : Bits m → Bits n}
+    (h : Increase k v f g) (h' : Nof (f k) v) :
+    sum f + v.toNat = sum g := by
+  induction m with
+  | zero =>
+    cases k; simp [sum_zero]
+    rw [← Bits.toNat_add_eq_of_nof _ _ h']
+    apply congr_arg _ <| (h ⦃⦄).left nil_eq_nil
+  | succ m ih =>
+    match k with
+    | b +> k =>
+      rcases frel_succ h with ⟨h_frel, h_eq⟩
+      rw [sum_succ_with b, sum_succ_with b, h_eq]
+      conv => lhs; lhs; rw [Nat.add_comm]
+      rw [Nat.add_assoc, ih h_frel h', Nat.add_comm]
+
+lemma add_le_sum_of_ne {m n} (f : Bits m → Bits n) {xs ys : Bits m}
+    (h : xs ≠ ys) : (f xs).toNat + (f ys).toNat ≤ sum f := by
+  induction m with
+  | zero => cases h nil_eq_nil
+  | succ m ih =>
+    match xs, ys with
+    | x +> xs, y +> ys =>
+      rw [sum_succ];
+      rcases Bool.zero_or_one x with h | h <;> cases h <;>
+      rcases Bool.zero_or_one y with h | h <;> cases h <;> simp at h
+      · apply @Nat.le_trans _ (sum (comp f 0)) _ _ (Nat.le_add_right _ _)
+        apply @ih (comp f 0) _ _ h
+      · apply Nat.add_le_add (@le_sum _ _ (comp f 0) _) (@le_sum _ _ (comp f 1) _)
+      · rw [Nat.add_comm]
+        apply Nat.add_le_add (@le_sum _ _ (comp f 0) _) (@le_sum _ _ (comp f 1) _)
+      · apply @Nat.le_trans _ (sum (comp f 1)) _ _ (Nat.le_add_left _ _)
+        apply @ih (comp f 1) _ _ h
+
+def Transfer {m n : Nat}
+    (b : Bits m → Bits n)
+    (kd : Bits m) (v : Bits n) (ki : Bits m)
+    (d : Bits m → Bits n) : Prop :=
+    v ≤ b kd ∧
+  ∃ c : Bits m → Bits n,
+    Decrease kd v b c ∧
+    Increase ki v c d
+
+lemma frel_of_frel {ξ υ} {x : ξ} {r s : υ → υ → Prop} {f g : ξ → υ}
+    (h : r (f x) (g x) → s (f x) (g x)) (h' : Frel x r f g) : Frel x s f g := by
+  intro x'; constructor <;> intro hx
+  · cases hx; exact h <| (h' x).left rfl
+  · exact (h' x').right hx
+
+lemma transfer_inv_sum {m n} {kd ki v} {b d : Bits m → Bits n}
+    (h' : SumNof b)
+    (h : Transfer b kd v ki d) : sum b = sum d := by
+  rcases h with ⟨h, c, hd, hi⟩
+
+  apply @Eq.trans _ _ (sum c + v.toNat)
+  · rw [← sum_sub_assoc hd h, Nat.sub_add_cancel]
+    apply Nat.le_trans (toNat_le_toNat _ _ h) le_sum
+  · apply @sum_add_assoc _ _ ki
+    apply frel_of_frel _ hi; intro h_eq; exact h_eq
+    by_cases hk : ki = kd
+    · rw [hk, ← (hd kd).left rfl]; simp [Nof]
+      rw [toNat_sub_eq_of_le _ _ h, Nat.sub_add_cancel (toNat_le_toNat _ _ h)]
+      apply toNat_lt_pow
+    · rw [← (hd ki).right (Ne.symm hk)]
+      apply lt_of_le_of_lt (Nat.le_trans _ <| add_le_sum_of_ne b hk) h'
+      apply Nat.add_le_add_left <| toNat_le_toNat _ _ h
+
+lemma transfer_inv_nof {m n} {kd ki v} {f g : Bits m → Bits n}
+    (h : Transfer f kd v ki g) (h' : SumNof f) : SumNof g := by
+  simp [SumNof]; rw [← transfer_inv_sum h' h]; apply h'
+
+
+open Bits
